theories/aneris_lang/state_interp/state_interp_local_coh.v
@@ -176,6 +176,29 @@ Section state_interpretation.
     iExists _; eauto.
   Qed.
 
+   Lemma local_state_coh_update_sblock a sh skt σ1 γs Sn r b :
+    let ip := ip_of_address a in
+    let S := <[ip := <[sh:= (skt<| sblock := b|>, r)]> Sn]>(state_sockets σ1) in
+    let σ2 := σ1 <| state_sockets := S |> in
+    state_sockets σ1 !! ip = Some Sn →
+    Sn !! sh = Some (skt, r) →
+    local_state_coh σ1 ip γs ∗ sh ↪[ip] skt ==∗
+    local_state_coh σ2 ip γs ∗ sh ↪[ip] (skt<|sblock := b|>).
+  Proof.
+    simpl. iIntros (??) "[Hstate Hsh]".
+    iDestruct "Hstate" as (h' S Hh Hs) "(#Hn & ? & Hsock)".
+    iDestruct "Hsh" as (γs') "[Hn' Hsh]".
+    iDestruct (mapsto_node_agree with "Hn Hn'") as %->.
+    simplify_eq.
+    iMod (gen_heap_light_update _ _ _ _ ((skt<|sblock := b|>, r).1)
+            with "Hsock Hsh") as "[Hsock' Hsh]".
+    iModIntro. iFrame. iSplitR "Hsh".
+    { iExists _, _. iFrame. rewrite lookup_insert //.
+      iSplit; first done. iSplit; first done.
+      rewrite fmap_insert /=. eauto with iFrame. }
+    iExists _; eauto.
+  Qed.
+
   Lemma big_sepM_local_state_coh_insert n γs γm σ :
     γm !! n = Some γs →
     local_state_coh σ n γs -∗
